ArkLib/Interaction/Oracle/Composition.lean
@@ -3,5 +3,5 @@ Copyright (c) 2026 ArkLib Contributors. All rights reserved.
 Released under Apache 2.0 license as described in the file LICENSE.
 Authors: Quang Dao
 -/
-import ArkLib.Interaction.Oracle.Core
-import ArkLib.Interaction.Oracle.Composition
+import ArkLib.Interaction.Oracle.Continuation
+import ArkLib.Interaction.Oracle.StateChain
